README.md
@@ -1,1 +1,62 @@
 # SortedList
+
+This repository aims to experiment with _formally verifying_ both **functional** and **imperative** programs using the Lean proof assistant.
+
+## Structure
+
+- `Main.lean` is a sample CLI for sorting lists. It also prints the unique values.
+- `Basic.lean` contains the definition of `Sorted`:
+    ```lean
+    abbrev Sorted (l : List Int) := Pairwise (· ≤ ·) l
+    ```
+- `Unique.lean` defines a naïve implementation of `unique : List Int -> List Int` recursively.
+- `Lemmas.lean` contains a lot of technical proofs about "sorted list theory"
+- `SortedList.lean` defines a `SortedList` as a subtype of lists:
+    ```lean
+    def SortedList := { l : List Int // l.Sorted }
+    ```
+    along with some API for sorted lists
+- `Decidable.lean` investigates how to decide when a list is sorted and its implications.
+- `Invariant.lean` experiments with the new Std.Do API.
+- `Imperative.lean` defines `unique` as an imperative program:
+    ```lean
+    def unique (xs : List Int) : Id (List Int) := do
+        let mut c : Option Int := none -- previous x in the list
+        let mut out := [] -- output of the function
+
+        for x in xs do
+            if some x != c then
+            out := out ++ [x]
+            c := some x
+
+        out
+    ```
+    and proves that it satisfies the following specification:
+    ```lean
+    ⦃⌜Sorted l⌝⦄ unique l ⦃⇓r => l ⊆ r ∧ StrictSorted r⦄
+    ```
+    which states that given a sorted list as input, `unique` returns a list with the following properties:
+    - every element in the input is in the output, and
+    - the output is strictly increasing (or equivalently, doesn't contain duplicates and is sorted).
+
+## Getting started
+
+1. Install Lean (`nix-shell -p elan` and `elan default stable`)
+2. Run `lake exe sortedlist`
+
+Sample run:
+
+```
+1 1 2 2 3
+Your input: [1, 1, 2, 2, 3]
+Unique elements: [1, 2, 3]
+1 2 3 4 1
+Your input: [1, 2, 3, 4, 1]
+Input was not sorted at index 4
+Your input (sorted): [1, 1, 2, 3, 4]
+Unique elements: [1, 2, 3, 4]
+```
+
+## Inspiration
+
+The imperative aspect is inspired by the very interesting blog post by Markus Himmel: [My first verified (imperative) program](https://markushimmel.de/blog/my-first-verified-imperative-program/).
